pulse/src/syntax_extension/PulseSyntaxWrapper.fsti
@@ -64,5 +64,6 @@ val comp_pre (c:comp) : term
 val comp_post (c:comp) : term
 
 val print_exn (e:exn) : string
+val term_to_string (env:FStar.TypeChecker.Env.env) (_:term) : either string string
 val st_term_to_string (env:FStar.TypeChecker.Env.env) (_:st_term) : either string string
 val comp_to_string (env:FStar.TypeChecker.Env.env) (_:comp) : either string string
